updated cam.dfy

cam.dfy
@@ -8,29 +8,31 @@
 
 
 datatype CAM = CAM(id:int,seqno:int, time:int, heading:int, speed:int, position:int)
+//Main method to get everything going
+
 // Min and Max CAM generation times in ms
 const T_GenCamMin := 100;
 const T_GenCamMax := 1000;
 
-const N_GenCamDefault := 3;
 const N_GenCamMax := 3;
+const N_GenCamDefault := N_GenCamMax;
 
 // Thresholds
 const headingthreshold := 4;
 const speedthreshold := 4;
 const posthreshold := 0.5 as real;
 
-const MaxTime := 5000; // How many ms to run simulation for
+const MaxMsgs := 100; // Max number of messages to verify for
 
-//Main method to get everything going
 method Main()
 {
   var carNo := 10;
-  var T_CheckCamGen := 10; // Every 10ms
-  var T_GenCam_DCC := 500; // Every 500ms, minimum time interval between two consecutive CAM generations 
+  var SleepInterval := 3;
+  var TxInterval := 5;
   var c := 0;
   
-  //for testing  
+  //for receive
+  
   var prev := new CAM [3];
   prev[0] := CAM(1,0,1,2,3,4);//for testing
   prev[1] := CAM(1,1,2,3,4,5);
@@ -45,96 +47,119 @@ method Main()
   }
   
 }
-
-method sendCAM(T_CheckCamGen:int, T_GenCam_DCC:int, j:int) returns (msgs:seq<CAM>)
+method sendCAM(T_CheckCamGen:int, T_GenCam_DCC:int, j: int) returns (msgs:seq<CAM>, now:int)
   requires 0 < T_CheckCamGen <= T_GenCamMin;
   requires T_GenCamMin <= T_GenCam_DCC <= T_GenCamMax;
-  requires T_GenCam_DCC>0;
 
-  //At least one CAM is sent for every TxInterval
-  ensures |msgs|>=1; // at least one cam is sent
-  ensures MaxTime/T_GenCam_DCC <= |msgs|;
-  
+  ensures T_GenCam_DCC * |msgs| <= now <= T_GenCamMax * |msgs|;
+  ensures |msgs| >= 2 ==> forall i: int :: 1 <= i < |msgs| ==> T_GenCam_DCC <= (msgs[i].time - msgs[i-1].time) <= T_GenCamMax;
+  ensures |msgs| == MaxMsgs;
 {
   var T_GenCam := T_GenCamMax; // currently valid upper limit of the CAM generation interval
-  var N_GenCam := N_GenCamDefault; 
+  var T_GenCamNext := T_GenCam;
+  var N_GenCam := N_GenCamDefault;
   var trigger_two_count := 0;
   
-  var LastBroadcast := 0;
-  var LastBroadcastDiff := 0;
-  var seqno := 0;
-  var prevheading, prevspeed, prevpos;
-  var now, heading, speed, pos := 0,0,0,0;
-  
-  
-  msgs := [CAM(j,seqno,now,heading,speed,pos)]; // send an initial cam
-  
-  var headingold:bool, speedold:bool, posold: bool := false, false, false;
-  
-  var t := 0;
-  assert |msgs| >=1;
-  while(t < MaxTime)
-  decreases MaxTime-t;
-  invariant |msgs|>=1;
-  invariant LastBroadcastDiff >= T_GenCam_DCC && (headingold || speedold || posold || (LastBroadcastDiff >= T_GenCam_DCC && |msgs|>=1 ))  ==> CAM(j,seqno,now,heading,speed,pos) in msgs;
-  invariant t/T_GenCamMin >= 1 ==> |msgs| >= t/T_GenCamMin;
-  invariant t/T_GenCamMax >= 1 ==> |msgs| >= t/T_GenCamMax;
-  invariant trigger_two_count > 0 && LastBroadcastDiff >= T_GenCam_DCC && LastBroadcastDiff >= T_GenCam &&  t/T_GenCamMax >= 1 ==> |msgs| >= t/T_GenCamMax;
-  invariant 0 <= N_GenCam <= N_GenCamMax;
-  
-  { 
-    //Get the current time
-    now := t;
-    LastBroadcastDiff := now - LastBroadcast;
-    
-    //Get vehicle information
-    heading := GetHeading();
-    speed := GetSpeed();
-    pos := GetPosition();
-    
-    //Check if this information has changed
-    headingold := abs(heading - prevheading) >= headingthreshold;
-    speedold := abs(speed - prevspeed) >= speedthreshold;
-    posold := abs(pos - prevpos) >= posthreshold.Floor;
-    
-    //If any information has changed, or a CAM hasn't been sent recently, then send a CAM
-    if(LastBroadcastDiff >= T_GenCam_DCC || (headingold || speedold || posold || LastBroadcastDiff >= T_GenCam)){
-      seqno := (seqno + 1) % 256;
-      msgs := msgs + [CAM(j,seqno,now,heading,speed,pos)];
-      LastBroadcast := now;
-      
-      if ((headingold || speedold || posold)) { // Trigger 1
-        T_GenCam := LastBroadcastDiff;
-        trigger_two_count := 0; // Reset
-      }
-      else if (LastBroadcastDiff >= T_GenCam){ // Trigger 2
-        trigger_two_count := trigger_two_count + 1;
-        if (trigger_two_count == N_GenCam) {
-          T_GenCam := T_GenCamMax;
-          
-       }
-       
-     }
-     
-      //Set current values as old values
-      prevheading := heading;
-      prevspeed := speed;
-      prevpos := pos;
-    }   
-    t := t + T_CheckCamGen; // Sleep for a bit to advance time
- }
- return msgs;
-}
+  now := 0;
+  var LastBroadcast, PrevLastBroadcast := now, now;
 
+  var heading, speed, pos := GetHeading(now), GetSpeed(now), GetPosition(now);
+  var prevheading, prevspeed, prevpos, statechanged := -1, -1, -1, false;
+
+  var seqno := 0;
+  msgs := [];
+  var prevsent := msgs;
+
+  while (|msgs| < MaxMsgs)
+  decreases MaxMsgs - |msgs|;
+  invariant 0 <= |msgs| <= MaxMsgs;
+
+  // Check variables remain within valid ranges
+  invariant 0 < N_GenCam <= N_GenCamMax;
+  invariant T_GenCamMin <= T_GenCamNext <= T_GenCamMax;
+  invariant T_GenCamMin <= T_GenCam <= T_GenCamMax;
+
+  invariant 0 <= PrevLastBroadcast <= now;
+  invariant now == LastBroadcast;
+  invariant now - T_GenCamMax <= PrevLastBroadcast <= LastBroadcast;  
+
+  // Check that messages are sent often enough
+  invariant |msgs| >= 1 ==> msgs[|msgs|-1].time == LastBroadcast;
+  invariant |msgs| >= 2 ==> msgs[|msgs|-2].time == PrevLastBroadcast;
+
+  invariant now > 0 ==> T_GenCam_DCC <= LastBroadcast - PrevLastBroadcast <= T_GenCamMax;
+  
+  // Message sent conditions (don't test when entering the loop)
+  invariant now > 0 ==> CAM(j,seqno,now,heading,speed,pos) in msgs;
+  invariant now > 0 ==> |prevsent| + 1 == |msgs|;
+
+  invariant |msgs| >= 2 ==> forall i: int :: 1 <= i < |msgs| ==> T_GenCam_DCC <= (msgs[i].time - msgs[i-1].time) <= T_GenCamMax;
+
+  invariant T_GenCamMin * |msgs| <= T_GenCam_DCC * |msgs| <= now;
+  invariant now > 0 ==> now <= T_GenCamMax * |msgs|;
+  {
+    prevsent, PrevLastBroadcast := msgs, LastBroadcast;
+    T_GenCam := T_GenCamNext;
+    statechanged := false;
+
+    // Advance time to the earliest a CAM can be sent (T_CamGen_DCC used as congestion control)
+    now := now + T_GenCam_DCC;
+
+    // Find the time at which information has changed or we have waited T_GenCam
+    while (true)
+    decreases LastBroadcast + T_GenCam - now;
+    invariant now - LastBroadcast <= max(T_GenCam_DCC, T_GenCam);
+    {
+        // Get vehicle information
+        heading, speed, pos := GetHeading(now), GetSpeed(now), GetPosition(now);
+      
+        // Check if this information has changed
+        statechanged := abs(heading - prevheading) >= headingthreshold ||
+                        abs(speed - prevspeed) >= speedthreshold ||
+                        abs(pos - prevpos) >= posthreshold.Floor;
+        
+        if (statechanged || now - LastBroadcast >= T_GenCam)
+        {
+            break; // Don't sleep if we need to send a CAM
+        }
+        else
+        {
+            now := now + T_CheckCamGen; // Sleep for a bit to advance time
+        }
+    }
+
+    assert LastBroadcast + T_GenCam_DCC <= now <= LastBroadcast + T_GenCamMax;
+    
+    seqno := (seqno + 1) % 256;
+    msgs := msgs + [CAM(j,seqno,now,heading,speed,pos)];
+    
+    if (statechanged) { // Trigger 1
+      T_GenCamNext := now - LastBroadcast;
+      trigger_two_count := 0; // Reset
+    }
+    else if (now - LastBroadcast >= T_GenCam){ // Trigger 2
+      trigger_two_count := trigger_two_count + 1;
+      if (trigger_two_count == N_GenCam) {
+        T_GenCamNext := T_GenCamMax;
+      }
+    }
+
+    // Set current values as old values
+    LastBroadcast := now;
+    prevheading, prevspeed, prevpos := heading, speed, pos;
+  }
+  return msgs, now;
+}
 method receiveCAM(fromid:int, cams:seq<CAM>) returns ()
 requires 0 <= fromid < |cams|;
 requires fromid == cams[fromid].id;  //To check that the vehicle the message claims it was sent from was actually sent from that vehicle.
 {
-  if(Sign(Magnitude(cams[fromid].heading)) == - Sign(Magnitude(GetHeading())))
+  var now := Now();
+  if(Sign(Magnitude(cams[fromid].heading)) == - Sign(Magnitude(GetHeading(now))))
   {
     //Ignore cars travelling in the opposite direction to us
   }
- var speeddiff := GetSpeed() - cams[fromid].speed;
+ var speeddiff := GetSpeed(now) - cams[fromid].speed;
 
  //Negative speeddiff indicates that we are getting closer to the vehicle ahead of us so we may need to brake
  if (speeddiff < 0){
@@ -151,17 +176,17 @@ method Now() returns(n:int)
   //returns the current time
 }
 
-function method GetHeading() :int
+function method GetHeading(now: int) :int
 {
   20
 }
 
-function method GetSpeed():int
+function method GetSpeed(now: int):int
 {
   50
 }
 
-function method GetPosition():int
+function method GetPosition(now: int):int
 {
   10
 }
@@ -171,26 +196,44 @@ function method abs(x: int): int
    if x < 0 then -x else x
 }
 
-function method Magnitude(heading:int):int{
-  heading
-}
 
+method Sleep(SleepInterval:int) returns ()
+{}
 
-method Sleep(period:int) returns ()
-{
-  
-}
 
 function method hasOverflowed(s1:int, s2:int): bool{
   s1>s2
 }
 
-function method Sign(x:int):int{
-  if x < 0 then -1 else 1
+function method Sign(magnitude:int):int{
+  magnitude
+}
+
+function method Magnitude(heading:int):int{
+  heading
 }
 
 method Brake(s:int)  returns (deceleration:int)
 ensures 0<= deceleration <= 10; // 10 should be 9.81 but left it as 10 so that I could use ints for simplicity 
 { 
   deceleration := 8;
+
+}
+function method max(x: int, y: int): int
+{
+  if x < y then y else x
+}
+
+ 
+method sqrt (s:int) returns (r:int)
+requires s >= 0;
+ensures 0 <= r * r && r*r <= s && s < (r+1)*(r+1); 
+{
+  r := 0 ;
+  while ((r+1) * (r+1) <= s)
+  decreases s - (r+1) * (r+1);
+  invariant r*r <= s ;
+  {
+    r := r+1 ;
+  }
 }
